src/Transforms/laa.v
@@ -16,6 +16,8 @@ Require Import promotable_props.
 Require Import primitives.
 Require Import id_rhs_val.
 Require Import palloca_props.
+Require Import mem2reg.
+Require Import program_sim.
 
 Definition laa (lid: id) (cs2:cmds) (b:block) (pinfo:PhiInfo) : Prop :=         
 blockInFdefB b (PI_f pinfo) = true /\
@@ -31,7 +33,6 @@ exists cs1, exists cs3,
 
 Record LAAInfo (pinfo: PhiInfo) := mkLAAInfo {
   LAA_lid : id;
-  LAA_sid : id;
   LAA_tail : cmds;
   LAA_block : block;
   LAA_prop : laa LAA_lid LAA_tail LAA_block pinfo
@@ -74,7 +75,7 @@ List.Forall2
    match M1, M2 with
    | module_intro los1 nts1 Ps1, module_intro los2 nts2 Ps2 =>
        los1 = los2 /\ nts1 = nts2 /\ 
-       products_simulation pinfo laainfo Ps1 Ps1
+       products_simulation pinfo laainfo Ps1 Ps2
    end) S1 S2.
 
 Definition phis_simulation (pinfo: PhiInfo) (laainfo: LAAInfo pinfo) (f1:fdef)
@@ -541,6 +542,171 @@ Transparent inscope_of_tmn inscope_of_cmd.
 
 Qed.
 *)
+
+Lemma find_st_ld__laainfo: forall l0 ps0 cs0 tmn0 v cs (pinfo:PhiInfo) dones
+  (Hst : ret inr (v, cs) = find_init_stld cs0 (PI_id pinfo) dones)
+  (i1 : id) (Hld : ret inl i1 = find_next_stld cs (PI_id pinfo))
+  (HBinF : blockInFdefB (block_intro l0 ps0 cs0 tmn0) (PI_f pinfo) = true),
+  v = [! pinfo !] /\
+  exists laainfo:LAAInfo pinfo,
+    LAA_lid pinfo laainfo = i1 /\
+    LAA_block pinfo laainfo = (block_intro l0 ps0 cs0 tmn0).
+Admitted.
+
+Lemma s_genInitState__laa_State_simulation: forall pinfo laainfo S1 S2 main 
+  VarArgs cfg2 IS2,
+  system_simulation pinfo laainfo S1 S2 ->
+  Opsem.s_genInitState S2 main VarArgs Mem.empty = ret (cfg2, IS2) ->
+  exists cfg1, exists IS1,
+    Opsem.s_genInitState S1 main VarArgs Mem.empty = ret (cfg1, IS1) /\
+    State_simulation pinfo laainfo cfg1 IS1 cfg2 IS2.
+Admitted.
+
+Lemma s_isFinialState__laa_State_simulation: forall pinfo laainfo cfg1 FS1 cfg2 
+  FS2 r (Hstsim : State_simulation pinfo laainfo cfg1 FS1 cfg2 FS2)
+  (Hfinal: s_isFinialState cfg2 FS2 = ret r),
+  s_isFinialState cfg1 FS1 = ret r.
+Admitted.
+
+Lemma opsem_s_isFinialState__laa_State_simulation: forall 
+  pinfo laainfo cfg1 FS1 cfg2 FS2  
+  (Hstsim : State_simulation pinfo laainfo cfg1 FS1 cfg2 FS2),
+  Opsem.s_isFinialState FS1 = Opsem.s_isFinialState FS2.
+Admitted.
+
+Lemma undefined_state__laa_State_simulation: forall pinfo laainfo cfg1 St1 cfg2 
+  St2 (Hstsim : State_simulation pinfo laainfo cfg1 St1 cfg2 St2),
+  OpsemPP.undefined_state cfg1 St1 -> OpsemPP.undefined_state cfg2 St2.
+Admitted.
+
+Lemma sop_star__laa_State_simulation: forall pinfo laainfo cfg1 IS1 cfg2 IS2 tr
+  FS2 (Hwfpi: WF_PhiInfo pinfo) (Hwfpp: OpsemPP.wf_State cfg1 IS1) 
+  (HwfS1: id_rhs_val.wf_State (value_id (LAA_lid pinfo laainfo)) 
+           [! pinfo !] (PI_f pinfo) cfg1 IS1)
+  (Hstsim : State_simulation pinfo laainfo cfg1 IS1 cfg2 IS2)
+  (Hopstar : Opsem.sop_star cfg2 IS2 FS2 tr),
+  exists FS1, Opsem.sop_star cfg1 IS1 FS1 tr /\ 
+    State_simulation pinfo laainfo cfg1 FS1 cfg2 FS2.
+Proof.
+  intros.
+  generalize dependent cfg1.
+  generalize dependent IS1.
+  induction Hopstar; intros.
+    exists IS1. split; auto.
+
+    assert (J:=Hwfpp).
+    apply OpsemPP.progress in J; auto.
+    destruct J as [Hfinal1 | [[IS1' [tr0 Hop1]] | Hundef1]].
+      apply opsem_s_isFinialState__laa_State_simulation in Hstsim.
+      rewrite Hstsim in Hfinal1.
+      contradict H; eauto using s_isFinialState__stuck.
+
+      eapply laa_is_sim in Hstsim; eauto.
+      destruct Hstsim as [Hstsim EQ]; subst.
+      assert (OpsemPP.wf_State cfg1 IS1') as Hwfpp'.
+        admit. (* wf pp *)
+      assert (id_rhs_val.wf_State (value_id (LAA_lid pinfo laainfo))
+               [! pinfo !] (PI_f pinfo) cfg1 IS1') as HwfS1'.
+        admit. (* wf pp *)
+      eapply IHHopstar in Hstsim; eauto.
+      destruct Hstsim as [FS1 [Hopstar1 Hstsim]].
+      exists FS1.
+      split; eauto.
+
+      eapply undefined_state__laa_State_simulation in Hstsim; eauto.
+      contradict H; eauto using undefined_state__stuck.
+Qed.
+
+Lemma sop_div__laa_State_simulation: forall pinfo laainfo cfg1 IS1 cfg2 IS2 tr
+  (Hwfpi: WF_PhiInfo pinfo) (Hwfpp: OpsemPP.wf_State cfg1 IS1) 
+  (HwfS1: id_rhs_val.wf_State (value_id (LAA_lid pinfo laainfo)) 
+            [! pinfo !] (PI_f pinfo) cfg1 IS1)
+  (Hstsim : State_simulation pinfo laainfo cfg1 IS1 cfg2 IS2)
+  (Hopstar : Opsem.sop_diverges cfg2 IS2 tr),
+  Opsem.sop_diverges cfg1 IS1 tr.
+Admitted.
+
+Lemma laa_sim: forall (los : layouts) (nts : namedts) (fh : fheader) 
+  (dones : list id) (pinfo : PhiInfo) (main : id) (VarArgs : list (GVsT DGVs))
+  (bs1 : list block) (l0 : l) (ps0 : phinodes) (cs0 : cmds) (tmn0 : terminator)
+  (bs2 : list block) (Ps1 : list product) (Ps2 : list product) (v : value)
+  (cs : cmds) 
+  (Hst : ret inr (v, cs) = find_init_stld cs0 (PI_id pinfo) dones)
+  (i1 : id) (Hld : ret inl i1 = find_next_stld cs (PI_id pinfo))
+  (Heq: PI_f pinfo = fdef_intro fh (bs1 ++ block_intro l0 ps0 cs0 tmn0 :: bs2))
+  (Hwfpi: WF_PhiInfo pinfo) 
+  (HwfS : 
+     wf_system nil
+       [module_intro los nts 
+         (Ps1 ++ 
+          product_fdef 
+            (fdef_intro fh (bs1 ++ block_intro l0 ps0 cs0 tmn0 :: bs2))
+          :: Ps2)]),
+  program_sim
+     [module_intro los nts
+        (Ps1 ++
+         product_fdef
+           (subst_fdef i1 v
+              (fdef_intro fh (bs1 ++ block_intro l0 ps0 cs0 tmn0 :: bs2)))
+         :: Ps2)]
+     [module_intro los nts
+        (Ps1 ++
+         product_fdef
+           (fdef_intro fh (bs1 ++ block_intro l0 ps0 cs0 tmn0 :: bs2)) :: Ps2)]
+     main VarArgs.
+Proof.
+  intros.
+  assert (blockInFdefB (block_intro l0 ps0 cs0 tmn0) (PI_f pinfo) = true)
+    as HBinF.
+    rewrite Heq. simpl. apply InBlocksB_middle.
+  eapply find_st_ld__laainfo in HBinF; eauto.
+  destruct HBinF as [EQ [laainfo [J1 J2]]]; subst.
+  assert (Huniq:=HwfS). apply wf_system__uniqSystem in Huniq; auto.
+  assert (system_simulation pinfo laainfo
+     [module_intro los nts
+        (Ps1 ++
+         product_fdef
+           (fdef_intro fh (bs1 ++ block_intro l0 ps0 cs0 tmn0 :: bs2)) :: Ps2)]
+     [module_intro los nts
+        (Ps1 ++
+         product_fdef
+           (subst_fdef (LAA_lid pinfo laainfo) [! pinfo !]
+              (fdef_intro fh (bs1 ++ block_intro l0 ps0 cs0 tmn0 :: bs2)))
+         :: Ps2)]) as Hssim.
+    unfold system_simulation.
+    constructor; auto.
+    repeat split; auto.
+    unfold products_simulation.
+    simpl in Huniq. destruct Huniq as [[_ [_ Huniq]] _].
+    apply uniq_products_simulation; auto.
+  constructor.
+    intros tr t Hconv.
+    inv Hconv.
+    eapply s_genInitState__laa_State_simulation in H; eauto.
+    destruct H as [cfg1 [IS1 [Hinit Hstsim]]].    
+    assert (OpsemPP.wf_State cfg1 IS1) as Hwfst. 
+      eapply s_genInitState__opsem_wf; eauto.
+    assert (id_rhs_val.wf_State (value_id (LAA_lid pinfo laainfo))
+              [! pinfo !] (PI_f pinfo) cfg1 IS1) as Hisrhsval.
+      eapply s_genInitState__id_rhs_val; eauto.
+    eapply sop_star__laa_State_simulation in Hstsim; eauto.
+    destruct Hstsim as [FS1 [Hopstar1 Hstsim']].
+    eapply s_isFinialState__laa_State_simulation in Hstsim'; eauto.
+    econstructor; eauto.
+
+    intros tr Hdiv.
+    inv Hdiv.
+    eapply s_genInitState__laa_State_simulation in H; eauto.
+    destruct H as [cfg1 [IS1 [Hinit Hstsim]]].  
+    assert (OpsemPP.wf_State cfg1 IS1) as Hwfst. 
+      eapply s_genInitState__opsem_wf; eauto.
+    assert (id_rhs_val.wf_State (value_id (LAA_lid pinfo laainfo))
+              [! pinfo !] (PI_f pinfo) cfg1 IS1) as Hisrhsval.
+      eapply s_genInitState__id_rhs_val; eauto.
+    eapply sop_div__laa_State_simulation in Hstsim; eauto.
+    destruct Hstsim as [FS1 Hopdiv1].
+    econstructor; eauto.
+Qed.
 
 (*****************************)
 (*
