src/Transforms/mem2reg_correct.v
@@ -4,6 +4,7 @@ Add LoadPath "../Vellvm/compcert".
 Add LoadPath "../Vellvm/GraphBasics".
 Add LoadPath "../Vellvm".
 Add LoadPath "../../../theory/metatheory_8.3".
+Add LoadPath "../SoftBound".
 Require Import vellvm.
 Require Import Kildall.
 Require Import ListSet.
@@ -17,68 +18,17 @@ Require Import primitives.
 Require Import palloca_props.
 Require Import mem2reg.
 Require Import memory_props.
-
-(* opsem should use this definition *)
-Definition s_isFinialState (cfg:OpsemAux.Config) (state:@Opsem.State DGVs) 
-  : option GenericValue :=
-match state with
-| (Opsem.mkState ((Opsem.mkEC _ _ nil (insn_return_void _) _ _)::nil) _ ) => 
-    const2GV (OpsemAux.CurTargetData cfg) (OpsemAux.Globals cfg) 
-      (const_int Size.One (INTEGER.of_Z 1%Z 1%Z false))
-| (Opsem.mkState ((Opsem.mkEC _ _ nil (insn_return _ _ v) lc _)::nil) _ ) => 
-    Opsem.getOperandValue (OpsemAux.CurTargetData cfg) v lc 
-      (OpsemAux.Globals cfg)
-| _ => None
-end.
-
-(* opsem should use this definition *)
-Inductive s_converges : 
-  system -> id -> list (GVsT DGVs) -> trace -> GenericValue -> Prop :=
-| s_converges_intro : forall (s:system) (main:id) (VarArgs:list (GVsT DGVs))    
-                              cfg (IS FS:Opsem.State) r tr,
-  Opsem.s_genInitState s main VarArgs Mem.empty = Some (cfg, IS) ->
-  Opsem.sop_star cfg IS FS tr ->
-  s_isFinialState cfg FS = Some r ->
-  s_converges s main VarArgs tr r
-.
-
-Definition stuck_state (cfg:OpsemAux.Config) (st:@Opsem.State DGVs) : Prop :=
-~ exists st', exists tr, Opsem.sInsn cfg st st' tr.
-
-(* opsem should use this definition *)
-Inductive s_goeswrong : 
-  system -> id -> list (GVsT DGVs) -> trace -> @Opsem.State DGVs  -> Prop :=
-| s_goeswrong_intro : forall (s:system) (main:id) (VarArgs:list (GVsT DGVs)) 
-                              cfg (IS FS:Opsem.State) tr,
-  Opsem.s_genInitState s main VarArgs Mem.empty = Some (cfg, IS) ->
-  Opsem.sop_star cfg IS FS tr ->
-  stuck_state cfg FS ->
-  ~ Opsem.s_isFinialState FS ->
-  s_goeswrong s main VarArgs tr FS
-.
-
-Inductive program_sim (P1 P2:system) (main:id) (VarArgs:list (GVsT DGVs)) :
-   Prop :=
-| program_sim_intro: 
-    (forall tr r, 
-      s_converges P1 main VarArgs tr r -> 
-      s_converges P2 main VarArgs tr r) -> 
-    (forall Tr, 
-      Opsem.s_diverges P1 main VarArgs Tr -> 
-      Opsem.s_diverges P2 main VarArgs Tr) ->
-    program_sim P1 P2 main VarArgs
-.
+Require Import program_sim.
+Require Import las.
+Require Import laa.
+Require Import dae.
+Require Import dse.
+Require Import die.
+Require Import sas.
+Require Import phiplacement_bsim.
 
 (* We are proving the macro-based m2r pass *)
 Parameter does_macro_m2r_is_true: mem2reg.does_macro_m2r tt = true.
-
-Lemma program_sim_refl: forall P main VarArgs, program_sim P P main VarArgs.
-Admitted.
-
-Lemma program_sim_trans: forall P1 P2 P3 main VarArgs, 
-  program_sim P1 P2 main VarArgs -> program_sim P2 P3 main VarArgs -> 
-  program_sim P1 P3 main VarArgs.
-Admitted.
 
 Parameter print_reachablity_is_true: forall rd, print_reachablity rd = true.
 
@@ -86,81 +36,34 @@ Parameter does_phi_elim_is_true: does_phi_elim tt = true.
 
 Parameter does_stld_elim_is_true: does_stld_elim tt = true.
 
-Lemma phinodes_placement_sim: forall rd f Ps1 Ps2 los nts main VarArgs pid ty al
-  l0 ps0 cs0 tmn0 dones (Hreach: ret rd = dtree.reachablity_analysis f)
-  (Hentry: getEntryBlock f = Some (block_intro l0 ps0 cs0 tmn0))
-  (Hfind: find_promotable_alloca f cs0 dones = Some (pid, ty, al)),
-  program_sim
-    [module_intro los nts 
-      (Ps1 ++ 
-       product_fdef (phinodes_placement f rd pid ty al (successors f)
-                    (make_predecessors (successors f))) :: Ps2)]
-    [module_intro los nts (Ps1 ++ product_fdef f :: Ps2)]
-    main VarArgs.
-Admitted.
-
-Lemma elim_stld_cmds_unchanged: forall f' dones' f cs0 pid dones,
-  (f', false, dones') = elim_stld_cmds f cs0 pid dones ->
-  f' = f.
-Proof.
-  intros.
-  unfold elim_stld_cmds in H.
-  destruct (find_init_stld cs0 pid dones) as [[[[]]|[]]|].
-    destruct (find_next_stld c pid) as [[|[]]|]; inv H.
-    destruct (find_next_stld c pid) as [[|[]]|]; inv H.
-    inv H; auto.
-Qed.
-
-Lemma remove_fdef_sim: forall f pid los nts Ps1 Ps2 main VarArgs,
-  used_in_fdef pid f = false ->
-  program_sim
-    [module_intro los nts 
-      (Ps1 ++  product_fdef (remove_fdef pid f) :: Ps2)]
-    [module_intro los nts (Ps1 ++ product_fdef f :: Ps2)]
-    main VarArgs.
-Admitted.
-
-Lemma las_sim: forall (los : layouts) (nts : namedts) (fh : fheader) 
-  (dones : list id) (pid : id) (main : id) (VarArgs : list (GVsT DGVs))
-  (bs1 : list block) (l0 : l) (ps0 : phinodes) (cs0 : cmds) (tmn0 : terminator)
-  (bs2 : list block) (Ps1 : list product) (Ps2 : list product) (i0 : id)
-  (v : value) (cs : cmds) 
-  (Hst : ret inl (i0, v, cs) = find_init_stld cs0 pid dones)
-  (i1 : id) (Hld : ret inl i1 = find_next_stld cs pid),
-  program_sim
-    [module_intro los nts
-      (Ps1 ++
-       product_fdef
-         (subst_fdef i1 v
-           (fdef_intro fh (bs1 ++ block_intro l0 ps0 cs0 tmn0 :: bs2))) :: Ps2)]
-    [module_intro los nts
-       (Ps1 ++
-        product_fdef
-          (fdef_intro fh (bs1 ++ block_intro l0 ps0 cs0 tmn0 :: bs2)) :: Ps2)]
-    main VarArgs.
-Proof.
-
-Admitted.
-
 Lemma las_die_sim: forall (los : layouts) (nts : namedts) (fh : fheader) 
-  (dones : list id) (pid : id) (main : id) (VarArgs : list (GVsT DGVs))
+  (dones : list id) (pinfo: PhiInfo) (main : id) (VarArgs : list (GVsT DGVs))
   (bs1 : list block) (l0 : l) (ps0 : phinodes) (cs0 : cmds) (tmn0 : terminator)
   (bs2 : list block) (Ps1 : list product) (Ps2 : list product) (i0 : id)
   (v : value) (cs : cmds) 
-  (Hst : ret inl (i0, v, cs) = find_init_stld cs0 pid dones)
-  (i1 : id) (Hld : ret inl i1 = find_next_stld cs pid),
+  (Hst : ret inl (i0, v, cs) = find_init_stld cs0 (PI_id pinfo) dones)
+  (i1 : id) (Hld : ret inl i1 = find_next_stld cs (PI_id pinfo))
+  (Heq: PI_f pinfo = fdef_intro fh (bs1 ++ block_intro l0 ps0 cs0 tmn0 :: bs2))
+  (Hwfpi: WF_PhiInfo pinfo) 
+  (HwfS : 
+     wf_system nil
+       [module_intro los nts 
+         (Ps1 ++ 
+          product_fdef 
+            (fdef_intro fh (bs1 ++ block_intro l0 ps0 cs0 tmn0 :: bs2))
+          :: Ps2)]),
   program_sim
     [module_intro los nts
       (Ps1 ++
        product_fdef
          (fdef_intro fh
            (List.map (remove_block i1)
-             (List.map (subst_block i1 v)
+             (List.map (subst_block i1 v) 
                (bs1 ++ block_intro l0 ps0 cs0 tmn0 :: bs2)))) :: Ps2)]
-    [module_intro los nts
-       (Ps1 ++
-        product_fdef
-          (fdef_intro fh (bs1 ++ block_intro l0 ps0 cs0 tmn0 :: bs2)) :: Ps2)]
+    [module_intro los nts 
+      (Ps1 ++ 
+       product_fdef (fdef_intro fh (bs1 ++ block_intro l0 ps0 cs0 tmn0 :: bs2))::
+       Ps2)]
     main VarArgs.
 Proof.
   intros.
@@ -181,40 +84,30 @@ Proof.
            (subst_fdef i1 v
               (fdef_intro fh (bs1 ++ block_intro l0 ps0 cs0 tmn0 :: bs2))) :: 
          Ps2)]).
-    apply remove_fdef_sim.
-      admit. (* subst i --> dead i *)  
-
-      eapply las_sim; eauto.
+    destruct (@subst_fdef__diinfo 
+      (fdef_intro fh (bs1 ++ block_intro l0 ps0 cs0 tmn0 :: bs2)) i1 v) as 
+      [diinfo [J1 J2]].
+    eapply die_sim; eauto.
+      admit. (* subst pres wfs *)  
+    eapply las_sim; eauto.
 Qed.
 
-Lemma laa_sim: forall (los : layouts) (nts : namedts) (fh : fheader) 
-  (dones : list id) (pid : id) (main : id) (VarArgs : list (GVsT DGVs))
-  (bs1 : list block) (l0 : l) (ps0 : phinodes) (cs0 : cmds) (tmn0 : terminator)
-  (bs2 : list block) (Ps1 : list product) (Ps2 : list product) (v : value)
-  (cs : cmds) 
-  (Hst : ret inr (v, cs) = find_init_stld cs0 pid dones)
-  (i1 : id) (Hld : ret inl i1 = find_next_stld cs pid),
-  program_sim
-     [module_intro los nts
-        (Ps1 ++
-         product_fdef
-           (subst_fdef i1 v
-              (fdef_intro fh (bs1 ++ block_intro l0 ps0 cs0 tmn0 :: bs2)))
-         :: Ps2)]
-     [module_intro los nts
-        (Ps1 ++
-         product_fdef
-           (fdef_intro fh (bs1 ++ block_intro l0 ps0 cs0 tmn0 :: bs2)) :: Ps2)]
-     main VarArgs.
-Admitted.
-
 Lemma laa_die_sim: forall (los : layouts) (nts : namedts) (fh : fheader) 
-  (dones : list id) (pid : id) (main : id) (VarArgs : list (GVsT DGVs))
+  (dones : list id) (pinfo : PhiInfo) (main : id) (VarArgs : list (GVsT DGVs))
   (bs1 : list block) (l0 : l) (ps0 : phinodes) (cs0 : cmds) (tmn0 : terminator)
   (bs2 : list block) (Ps1 : list product) (Ps2 : list product) (v : value)
   (cs : cmds) 
-  (Hst : ret inr (v, cs) = find_init_stld cs0 pid dones)
-  (i1 : id) (Hld : ret inl i1 = find_next_stld cs pid),
+  (Hst : ret inr (v, cs) = find_init_stld cs0 (PI_id pinfo) dones)
+  (i1 : id) (Hld : ret inl i1 = find_next_stld cs (PI_id pinfo))
+  (Heq: PI_f pinfo = fdef_intro fh (bs1 ++ block_intro l0 ps0 cs0 tmn0 :: bs2))
+  (Hwfpi: WF_PhiInfo pinfo) 
+  (HwfS : 
+     wf_system nil
+       [module_intro los nts 
+         (Ps1 ++ 
+          product_fdef 
+            (fdef_intro fh (bs1 ++ block_intro l0 ps0 cs0 tmn0 :: bs2))
+          :: Ps2)]),
   program_sim
     [module_intro los nts
       (Ps1 ++
@@ -247,40 +140,30 @@ Proof.
            (subst_fdef i1 v
               (fdef_intro fh (bs1 ++ block_intro l0 ps0 cs0 tmn0 :: bs2))) :: 
          Ps2)]).
-    apply remove_fdef_sim.
-      admit. (* subst i --> dead i *)  
+    destruct (@subst_fdef__diinfo 
+      (fdef_intro fh (bs1 ++ block_intro l0 ps0 cs0 tmn0 :: bs2)) i1 v) as 
+      [diinfo [J1 J2]].
+    eapply die_sim; eauto.
+      admit. (* subst pres wfS *)  
 
-      eapply laa_sim; eauto.
+    eapply laa_sim; eauto.
 Qed.
 
-Lemma sas_sim: forall (los : layouts) (nts : namedts) (fh : fheader) 
-  (dones : list id) (pid : id) (main : id) (VarArgs : list (GVsT DGVs))
-  (bs1 : list block) (l0 : l) (ps0 : phinodes) (cs0 : cmds) (tmn0 : terminator)
-  (bs2 : list block) (Ps1 : list product) (Ps2 : list product) (i0 : id)
-  (v : value) (cs : cmds) 
-  (Hst1 : ret inl (i0, v, cs) = find_init_stld cs0 pid dones)
-  (i1 : id) (v0 : value)
-  (Hst2 : ret inr (i1, v0) = find_next_stld cs pid),
-  program_sim
-    [module_intro los nts
-      (Ps1 ++
-       product_fdef
-         (fdef_intro fh
-           (List.map (remove_block i0)
-             (bs1 ++ block_intro l0 ps0 cs0 tmn0 :: bs2))) :: Ps2)]
-    [module_intro los nts
-      (Ps1 ++
-       product_fdef
-         (fdef_intro fh (bs1 ++ block_intro l0 ps0 cs0 tmn0 :: bs2)) :: Ps2)]
-    main VarArgs.
-Admitted.
-
-Lemma elim_stld_cmds_sim: forall los nts fh dones pid f0 dones0 main VarArgs
-  bs1 l0 ps0 cs0 tmn0 bs2 Ps1 Ps2
+Lemma elim_stld_cmds_sim: forall los nts fh dones (pinfo:PhiInfo) f0 dones0 main 
+  VarArgs bs1 l0 ps0 cs0 tmn0 bs2 Ps1 Ps2
   (Hpass : (f0, true, dones0) =
-             elim_stld_cmds
-               (fdef_intro fh (bs1 ++ block_intro l0 ps0 cs0 tmn0 :: bs2)) cs0
-               pid dones),
+           elim_stld_cmds
+             (fdef_intro fh (bs1 ++ block_intro l0 ps0 cs0 tmn0 :: bs2)) cs0
+             (PI_id pinfo) dones)
+  (Heq: PI_f pinfo = fdef_intro fh (bs1 ++ block_intro l0 ps0 cs0 tmn0 :: bs2))
+  (Hwfpi: WF_PhiInfo pinfo) 
+  (HwfS : 
+     wf_system nil
+       [module_intro los nts 
+         (Ps1 ++ 
+          product_fdef 
+            (fdef_intro fh (bs1 ++ block_intro l0 ps0 cs0 tmn0 :: bs2))
+          :: Ps2)]),
   program_sim 
     [module_intro los nts (Ps1 ++ product_fdef f0 :: Ps2)]
     [module_intro los nts
@@ -291,25 +174,33 @@ Lemma elim_stld_cmds_sim: forall los nts fh dones pid f0 dones0 main VarArgs
 Proof.
   intros.
   unfold elim_stld_cmds in Hpass.
-  remember (find_init_stld cs0 pid dones) as R1.
+  remember (find_init_stld cs0 (PI_id pinfo) dones) as R1.
   destruct R1 as [[[[]]|[]]|]; tinv Hpass.
-    remember (find_next_stld c pid) as R2.
+    remember (find_next_stld c (PI_id pinfo)) as R2.
     destruct R2 as [[|[]]|]; inv Hpass.
       eapply las_die_sim; eauto.
       eapply sas_sim; eauto.
       apply program_sim_refl.
 
-    remember (find_next_stld c pid) as R2.
+    remember (find_next_stld c (PI_id pinfo)) as R2.
     destruct R2 as [[|[]]|]; inv Hpass.
       eapply laa_die_sim; eauto.
       apply program_sim_refl.
       apply program_sim_refl.
 Qed.
 
-Lemma elim_stld_blocks_sim_aux: forall los nts fh dones pid f0 dones0 main 
-  VarArgs Ps1 Ps2 flag bs2 bs1 
-  (Hpass:elim_stld_blocks (fdef_intro fh (bs1++bs2)) bs2 pid dones = 
-    (f0, flag, dones0)),
+Lemma elim_stld_blocks_sim_aux: forall los nts fh dones (pinfo:PhiInfo) f0 dones0
+  main VarArgs Ps1 Ps2 flag bs2 bs1 
+  (Hpass:elim_stld_blocks (fdef_intro fh (bs1++bs2)) bs2 (PI_id pinfo) dones = 
+    (f0, flag, dones0))
+  (Heq: PI_f pinfo = fdef_intro fh (bs1 ++ bs2))
+  (Hwfpi: WF_PhiInfo pinfo) 
+  (HwfS : 
+     wf_system nil
+       [module_intro los nts 
+         (Ps1 ++ 
+          product_fdef 
+            (fdef_intro fh (bs1 ++ bs2)) :: Ps2)]),
   program_sim
     [module_intro los nts                                                      
       (Ps1 ++ 
@@ -324,19 +215,26 @@ Proof.
     destruct a as [l0 ps0 cs0 tmn0].
     remember 
       (elim_stld_cmds 
-        (fdef_intro fh (bs1 ++ block_intro l0 ps0 cs0 tmn0 :: bs2)) cs0 pid dones) 
-      as R.
+        (fdef_intro fh (bs1 ++ block_intro l0 ps0 cs0 tmn0 :: bs2)) 
+          cs0 (PI_id pinfo) dones) as R.
     destruct R as [[f' []] dones']; inv Hpass; auto.
       eapply elim_stld_cmds_sim; eauto.
 
       apply elim_stld_cmds_unchanged in HeqR. subst. 
       rewrite_env ((bs1 ++ [block_intro l0 ps0 cs0 tmn0]) ++ bs2) in H0.
-      apply IHbs2 in H0. simpl_env in H0. auto.
+      apply IHbs2 in H0; simpl_env in *; auto.
 Qed.
 
-Lemma elim_stld_blocks_sim: forall los nts fh dones pid f0 dones0 main 
-  VarArgs Ps1 Ps2 flag bs 
-  (Hpass:elim_stld_blocks (fdef_intro fh bs) bs pid dones = (f0, flag, dones0)),
+Lemma elim_stld_blocks_sim: forall los nts fh dones (pinfo:PhiInfo) f0 dones0 
+  main VarArgs Ps1 Ps2 flag bs 
+  (Hpass:elim_stld_blocks (fdef_intro fh bs) bs (PI_id pinfo) dones 
+           = (f0, flag, dones0))
+  (Heq: PI_f pinfo = fdef_intro fh bs)
+  (Hwfpi: WF_PhiInfo pinfo) 
+  (HwfS : 
+     wf_system nil
+       [module_intro los nts 
+         (Ps1 ++ product_fdef (fdef_intro fh bs) :: Ps2)]),
   program_sim
     [module_intro los nts                                                      
       (Ps1 ++ 
@@ -349,21 +247,25 @@ Proof.
   eapply elim_stld_blocks_sim_aux; eauto.
 Qed.
 
-Lemma elim_stld_sim: forall f1 dones1 f2 dones2 Ps1 Ps2 los nts main VarArgs pid
-  (Hpass: SafePrimIter.iterate _ (elim_stld_step pid) (f1, dones1) = 
-    (f2, dones2)),
+Lemma elim_stld_sim: forall f1 dones1 f2 dones2 Ps1 Ps2 los nts main VarArgs
+  pid (pinfo:PhiInfo) 
+  (Hpass: SafePrimIter.iterate _ (elim_stld_step pid) 
+    (f1, dones1) = (f2, dones2))
+  (Heq1: PI_f pinfo = f1) (Heq2: PI_id pinfo = pid)
+  (Hwfpi: WF_PhiInfo pinfo) 
+  (HwfS : wf_system nil [module_intro los nts (Ps1 ++ product_fdef f1 :: Ps2)]),
   program_sim
     [module_intro los nts (Ps1 ++ product_fdef f2 :: Ps2)]
     [module_intro los nts (Ps1 ++ product_fdef f1 :: Ps2)]
     main VarArgs.
 Proof.
-  intros.
+  intros. subst.
   set (P:=fun (re:(fdef * list id)) =>
           let '(f, _) := re in
           program_sim [module_intro los nts (Ps1 ++ product_fdef f :: Ps2)]
-           [module_intro los nts (Ps1 ++ product_fdef f1 :: Ps2)] main VarArgs
-      ).
-  assert (P (f1, dones1)) as HPf1.
+           [module_intro los nts (Ps1 ++ product_fdef (PI_f pinfo) :: Ps2)] 
+           main VarArgs).
+  assert (P (PI_f pinfo, dones1)) as HPf1.
     unfold P. apply program_sim_refl.
   apply SafePrimIter.iterate_prop with (P:=P) in Hpass; auto.
     unfold elim_stld_step.
@@ -371,7 +273,7 @@ Proof.
     destruct a as [f dones].
     unfold elim_stld_fdef.
     destruct f as [fh bs].
-    remember (elim_stld_blocks (fdef_intro fh bs) bs pid dones) as R.
+    remember (elim_stld_blocks (fdef_intro fh bs) bs (PI_id pinfo) dones) as R.
     destruct R as [[f0 flag0] dones0]; auto.
     assert (P (f0, dones0)) as HPf0.
       unfold P.
@@ -379,20 +281,14 @@ Proof.
            [module_intro los nts 
              (Ps1 ++ product_fdef (fdef_intro fh bs) :: Ps2)]); auto.
       eapply elim_stld_blocks_sim; eauto.
+        admit. (* PhiInfo is preserved *)
+        admit. (* wfS is preserved *)
     destruct flag0; auto.
 Qed.
 
-Lemma elim_dead_st_fdef_sim: forall f pid Ps1 Ps2 los nts main VarArgs,
-  load_in_fdef pid f = false ->
-  program_sim
-    [module_intro los nts 
-      (Ps1 ++  product_fdef (elim_dead_st_fdef f pid) :: Ps2)]
-    [module_intro los nts (Ps1 ++ product_fdef f :: Ps2)]
-    main VarArgs.
-Admitted.  
-
 Lemma macro_mem2reg_fdef_sim: forall rd f1 dones1 f2 dones2 Ps1 Ps2 los nts main
   VarArgs (Hreach: ret rd = dtree.reachablity_analysis f1)
+  (HwfS : wf_system nil [module_intro los nts (Ps1 ++ product_fdef f1 :: Ps2)])
   (Hiter: SafePrimIter.iterate (fdef * list id)
             (macro_mem2reg_fdef_step rd (successors f1)
               (make_predecessors (successors f1))) 
@@ -406,7 +302,7 @@ Proof.
   set (P:=fun (re:(fdef * list id)) =>
           let '(f, _) := re in
           program_sim [module_intro los nts (Ps1 ++ product_fdef f :: Ps2)]
-           [module_intro los nts (Ps1 ++ product_fdef f1 :: Ps2)] main VarArgs
+            [module_intro los nts (Ps1 ++ product_fdef f1 :: Ps2)] main VarArgs
       ).
   assert (P (f1, dones1)) as HPf1.
     unfold P. apply program_sim_refl.
@@ -418,7 +314,9 @@ Proof.
     remember (getEntryBlock f) as R.
     destruct R as [[l0 ps0 cs0 tmn0]|]; auto.
     remember (find_promotable_alloca f cs0 dones) as R.
-    destruct R as [[[pid ty] al]|]; auto.
+    destruct R as [[[[pid ty] num] al]|]; auto.
+    set (pinfo:=mkPhiInfo f rd pid ty num al).
+
     rewrite does_stld_elim_is_true.
       remember (SafePrimIter.iterate (fdef * list id) 
                  (elim_stld_step pid)
@@ -433,7 +331,13 @@ Proof.
             product_fdef 
                (phinodes_placement f rd pid ty al (successors f1)
                  (make_predecessors (successors f1))) :: Ps2)]).
-          eapply elim_stld_sim; eauto.
+          eapply elim_stld_sim with 
+            (pinfo:=mkPhiInfo (phinodes_placement f rd pid ty al (successors f1)
+                      (make_predecessors (successors f1))) rd pid ty num al); 
+            eauto.
+            admit. (* PhiInfo pres*)
+            admit. (* wfS pres*)
+
           apply program_sim_trans with (P2:=
             [module_intro los nts (Ps1 ++ product_fdef f :: Ps2)]); auto.
             assert (successors f1 = successors f) as EQ1. admit. rewrite EQ1.
@@ -442,24 +346,32 @@ Proof.
               admit. 
             rewrite EQ2 in Hreach.
             eapply phinodes_placement_sim; eauto.
+              admit. (* wfS pres *) 
        assert (P 
-                (if load_in_fdef pid f0 then f0 else elim_dead_st_fdef f0 pid,
+                (if load_in_fdef pid f0 then f0 else elim_dead_st_fdef pid f0,
                  nil)) as Pf.
          remember (load_in_fdef pid f0) as R.
          destruct R; auto.
          unfold P.
          apply program_sim_trans with (P2:=
            [module_intro los nts (Ps1 ++ product_fdef f0 :: Ps2)]); auto.
-         apply elim_dead_st_fdef_sim; auto.
+         apply dse_sim with (pinfo:=mkPhiInfo f0 rd pid ty num al); auto.
+           admit. (* WFPI pres *)
+           admit. (* wfS pres *)
        remember (used_in_fdef pid
-           (if load_in_fdef pid f0 then f0 else elim_dead_st_fdef f0 pid)) as R.
+           (if load_in_fdef pid f0 then f0 else elim_dead_st_fdef pid f0)) as R.
        destruct R; auto.
        apply program_sim_trans with (P2:=
          [module_intro los nts 
            (Ps1 ++ product_fdef 
                      (if load_in_fdef pid f0 then f0 
-                      else elim_dead_st_fdef f0 pid) :: Ps2)]); auto.
-       apply remove_fdef_sim; auto.
+                      else elim_dead_st_fdef pid f0) :: Ps2)]); auto.
+       eapply dae_sim with 
+         (pinfo:=mkPhiInfo 
+           (if load_in_fdef pid f0 then f0 else elim_dead_st_fdef pid f0)
+           rd pid ty num al); eauto.
+         admit. (* WFPI pres *)
+         admit. (* wfS pres *)
 Qed.
 
 Lemma eliminate_phis_sim: forall f Ps1 Ps2 los nts main VarArgs,
@@ -478,7 +390,8 @@ Axiom fix_temporary_fdef_sim: forall f1 f2 Ps1 Ps2 los nts main VarArgs
     main VarArgs.
 
 Lemma mem2reg_fdef_sim: forall (main : id) (VarArgs : list (GVsT DGVs))
-  (los : layouts) (nts : namedts) (f : fdef) (Ps2 Ps1 : products),
+  (los : layouts) (nts : namedts) (f : fdef) (Ps2 Ps1 : products)
+ (HwfS : wf_system nil [module_intro los nts (Ps1 ++ product_fdef f :: Ps2)]),
   program_sim
     [module_intro los nts (Ps1 ++ product_fdef (mem2reg_fdef f) :: Ps2)]
     [module_intro los nts (Ps1 ++ product_fdef f :: Ps2)]
@@ -514,7 +427,8 @@ Proof.
 Qed.
 
 Lemma mem2reg_run_sim_aux: forall (main : id) (VarArgs : list (GVsT DGVs))        
-  (los : layouts) (nts : namedts) (Ps2 Ps1: products),
+  (los : layouts) (nts : namedts) (Ps2 Ps1: products)
+  (HwfS : wf_system nil [module_intro los nts (Ps1 ++ Ps2)]),
   program_sim
     [module_intro los nts
       (Ps1 ++ List.map
@@ -539,9 +453,11 @@ Proof.
                      | _ => p
                      end) Ps2)]); auto.
     apply mem2reg_fdef_sim.
+      admit. (* wfS pres *)
 Qed.
 
-Lemma mem2reg_run_sim: forall (m:module) (main:id) (VarArgs:list (GVsT DGVs)),
+Lemma mem2reg_run_sim: forall (m:module) (main:id) (VarArgs:list (GVsT DGVs))
+  (HwfS : wf_system nil [m]),
   program_sim [mem2reg.run m] [m] main VarArgs.
 Proof.
   destruct m as [los nts Ps].
