src/Transforms/dae.v
@@ -21,6 +21,7 @@ Require Import sb_msim.
 Require Import sb_ds_trans_lib.
 Require Import sb_ds_gv_inject.
 Require Import sb_metadata.
+Require Import program_sim.
 
 Definition fdef_simulation (pinfo: PhiInfo) f1 f2 : Prop :=
   if (fdef_dec (PI_f pinfo) f1) then 
@@ -51,7 +52,7 @@ List.Forall2
    match M1, M2 with
    | module_intro los1 nts1 Ps1, module_intro los2 nts2 Ps2 =>
        los1 = los2 /\ nts1 = nts2 /\ 
-       products_simulation pinfo Ps1 Ps1
+       products_simulation pinfo Ps1 Ps2
    end) S1 S2.
 
 Definition is_alloca_in_EC (pinfo: PhiInfo) F1 (lc1:@Opsem.GVsMap DGVs) 
@@ -3429,6 +3430,144 @@ SCase "sExCall".
 
 Transparent inscope_of_tmn inscope_of_cmd.
 
+Qed.
+
+Lemma s_genInitState__dae_State_simulation: forall pinfo S1 S2 main VarArgs cfg2 
+  IS2,
+  system_simulation pinfo S1 S2 ->
+  Opsem.s_genInitState S2 main VarArgs Mem.empty = ret (cfg2, IS2) ->
+  exists maxb, exists mi, exists cfg1, exists IS1,
+    Opsem.s_genInitState S1 main VarArgs Mem.empty = ret (cfg1, IS1) /\
+    State_simulation pinfo maxb mi cfg1 IS1 cfg2 IS2 /\
+    sb_ds_gv_inject.wf_globals maxb (OpsemAux.Globals cfg1) /\
+    0 <= maxb /\
+    Promotability.wf_State maxb pinfo cfg1 IS1.
+Admitted.
+
+Lemma s_isFinialState__dae_State_simulation: forall maxb mi pinfo cfg1 FS1 cfg2 
+  FS2 r (Hstsim : State_simulation pinfo maxb mi cfg1 FS1 cfg2 FS2)
+  (Hfinal: s_isFinialState cfg2 FS2 = ret r),
+  s_isFinialState cfg1 FS1 = ret r.
+Admitted.
+
+Lemma opsem_s_isFinialState__dae_State_simulation: forall 
+  pinfo maxb mi cfg1 FS1 cfg2 FS2  
+  (Hstsim : State_simulation pinfo maxb mi cfg1 FS1 cfg2 FS2),
+  Opsem.s_isFinialState FS1 = Opsem.s_isFinialState FS2.
+Admitted.
+
+Lemma undefined_state__dae_State_simulation: forall pinfo maxb mi cfg1 St1 cfg2 
+  St2 (Hstsim : State_simulation pinfo maxb mi cfg1 St1 cfg2 St2),
+  OpsemPP.undefined_state cfg1 St1 -> OpsemPP.undefined_state cfg2 St2.
+Admitted.
+
+Lemma sop_star__dae_State_simulation: forall pinfo mi cfg1 IS1 cfg2 IS2 tr
+  FS2 (Hwfpi: WF_PhiInfo pinfo) (Hwfpp: OpsemPP.wf_State cfg1 IS1) maxb
+  (Hwfg: sb_ds_gv_inject.wf_globals maxb (OpsemAux.Globals cfg1))
+  (Hless: 0 <= maxb) (Hnuse: used_in_fdef (PI_id pinfo) (PI_f pinfo) = false)
+  (Hnoalias: Promotability.wf_State maxb pinfo cfg1 IS1)
+  (Hstsim : State_simulation pinfo maxb mi cfg1 IS1 cfg2 IS2)
+  (Hopstar : Opsem.sop_star cfg2 IS2 FS2 tr),
+  exists FS1, exists mi', Opsem.sop_star cfg1 IS1 FS1 tr /\ 
+    State_simulation pinfo maxb mi' cfg1 FS1 cfg2 FS2 /\
+    inject_incr mi mi'.
+Proof.
+  intros.
+  generalize dependent cfg1.
+  generalize dependent IS1.
+  generalize dependent mi.
+  induction Hopstar; intros.
+    exists IS1. exists mi. split; auto.
+
+    assert (J:=Hwfpp).
+    apply OpsemPP.progress in J; auto.
+    destruct J as [Hfinal1 | [[IS1' [tr0 Hop1]] | Hundef1]].
+      apply opsem_s_isFinialState__dae_State_simulation in Hstsim.
+      rewrite Hstsim in Hfinal1.
+      contradict H; eauto using s_isFinialState__stuck.
+
+      assert (OpsemPP.wf_State cfg1 IS1') as Hwfpp'.
+        admit. (* wf pp *)
+      assert (Promotability.wf_State maxb pinfo cfg1 IS1') as Hnoalias'.
+        admit. (* wf pp *)
+      eapply dae_is_sim in Hstsim; eauto.
+      destruct Hstsim as [Hstsim1 Hstsim2].
+      destruct (@removable_State_dec pinfo IS1) as [Hrm | Hnrm].
+        eapply Hstsim1 in Hrm; eauto.
+        destruct Hrm as [Hstsim EQ]; subst.
+        admit. (* we should do induction on the measure of State_simulation *)
+
+        eapply Hstsim2 in Hnrm; eauto.
+        destruct Hnrm as [mi' [Hstsim [EQ Hinc]]]; subst.
+        eapply IHHopstar in Hstsim; eauto.
+        destruct Hstsim as [FS1 [mi'' [Hopstar1 [Hstsim Hinc']]]].
+        exists FS1. exists mi''.
+        split; eauto.
+        split; eauto.
+          eapply inject_incr_trans; eauto.
+
+      eapply undefined_state__dae_State_simulation in Hstsim; eauto.
+      contradict H; eauto using undefined_state__stuck.
+Qed.
+
+Lemma sop_div__dae_State_simulation: forall pinfo cfg1 IS1 cfg2 IS2 tr
+  (Hwfpi: WF_PhiInfo pinfo) (Hwfpp: OpsemPP.wf_State cfg1 IS1) maxb mi
+  (Hwfg: sb_ds_gv_inject.wf_globals maxb (OpsemAux.Globals cfg1))
+  (Hless: 0 <= maxb) (Hnuse: used_in_fdef (PI_id pinfo) (PI_f pinfo) = false)
+  (Hnoalias: Promotability.wf_State maxb pinfo cfg1 IS1)
+  (Hstsim : State_simulation pinfo maxb mi cfg1 IS1 cfg2 IS2)
+  (Hopstar : Opsem.sop_diverges cfg2 IS2 tr),
+  Opsem.sop_diverges cfg1 IS1 tr.
+Admitted.
+     
+Lemma dae_sim: forall id0 f pinfo los nts Ps1 Ps2 main VarArgs
+  (Hwfpi: WF_PhiInfo pinfo)  
+  (HwfS: wf_system nil [module_intro los nts (Ps1 ++ product_fdef f :: Ps2)])
+  (Hnuse: used_in_fdef (PI_id pinfo) (PI_f pinfo) = false)
+  (Heq1: f = PI_f pinfo) (Heq2: id0 = PI_id pinfo),
+  program_sim
+    [module_intro los nts 
+      (Ps1 ++  product_fdef (remove_fdef id0 f) :: Ps2)]
+    [module_intro los nts (Ps1 ++ product_fdef f :: Ps2)]
+    main VarArgs.
+Proof.
+  intros. subst.
+  assert (Huniq:=HwfS). apply wf_system__uniqSystem in Huniq; auto.
+  assert (system_simulation pinfo
+    [module_intro los nts (Ps1 ++ product_fdef (PI_f pinfo) :: Ps2)]
+    [module_intro los nts
+      (Ps1 ++ product_fdef (remove_fdef (PI_id pinfo) (PI_f pinfo)) :: Ps2)])
+    as Hssim.
+    unfold system_simulation.
+    constructor; auto.
+    repeat split; auto.
+    unfold products_simulation.
+    simpl in Huniq. destruct Huniq as [[_ [_ Huniq]] _].
+    apply uniq_products_simulation; auto.
+
+  constructor.
+    intros tr t Hconv.
+    inv Hconv.
+    eapply s_genInitState__dae_State_simulation in H; eauto.
+    destruct H as 
+      [maxb [mi [cfg1 [IS1 [Hinit1 [Hstsim [Hwfg [Hless Hprom]]]]]]]]. 
+    assert (OpsemPP.wf_State cfg1 IS1) as Hwfst. 
+      eapply s_genInitState__opsem_wf; eauto.
+    eapply sop_star__dae_State_simulation in Hstsim; eauto.
+    destruct Hstsim as [FS1 [mi' [Hopstar1 [Hstsim' Hinc]]]].
+    eapply s_isFinialState__dae_State_simulation in Hstsim'; eauto.
+    econstructor; eauto.
+
+    intros tr Hdiv.
+    inv Hdiv.
+    eapply s_genInitState__dae_State_simulation in H; eauto.
+    destruct H as 
+      [maxb [mi [cfg1 [IS1 [Hinit1 [Hstsim [Hwfg [Hless Hprom]]]]]]]]. 
+    assert (OpsemPP.wf_State cfg1 IS1) as Hwfst. 
+      eapply s_genInitState__opsem_wf; eauto.
+    eapply sop_div__dae_State_simulation in Hstsim; eauto.
+    destruct Hstsim as [FS1 Hopdiv1].
+    econstructor; eauto.
 Qed.
 
 (*****************************)
