src/Transforms/sas.v
@@ -18,6 +18,7 @@ Require Import id_rhs_val.
 Require Import palloca_props.
 Require Import memory_props.
 Require Import mem2reg.
+Require Import program_sim.
 
 Definition sas (sid1 sid2: id) (v1 v2:value) (cs2:cmds) (b:block) 
   (pinfo:PhiInfo) : Prop :=         
@@ -76,7 +77,7 @@ List.Forall2
    match M1, M2 with
    | module_intro los1 nts1 Ps1, module_intro los2 nts2 Ps2 =>
        los1 = los2 /\ nts1 = nts2 /\ 
-       products_simulation pinfo sasinfo Ps1 Ps1
+       products_simulation pinfo sasinfo Ps1 Ps2
    end) S1 S2.
 
 Definition EC_simulation (pinfo: PhiInfo) (sasinfo: SASInfo pinfo) 
@@ -173,7 +174,19 @@ match St with
 | _ => False
 end.
 
-Lemma dse_is_sim : forall maxb pinfo (sasinfo: SASInfo pinfo) Cfg1 St1 Cfg2 St2
+Lemma removable_State_dec : forall pinfo sasinfo St,
+  removable_State pinfo sasinfo St \/ ~ removable_State pinfo sasinfo St.
+Proof.
+  destruct St. 
+  destruct ECS as [|[]]; auto.
+  destruct CurCmds; auto.
+  simpl.
+  destruct c; auto.
+  destruct (fdef_dec (PI_f pinfo) CurFunction); auto.
+  destruct (id_dec i0 (SAS_sid1 pinfo sasinfo)); auto.
+Qed.
+
+Lemma sas_is_sim : forall maxb pinfo (sasinfo: SASInfo pinfo) Cfg1 St1 Cfg2 St2
   (Hwfpi: WF_PhiInfo pinfo) 
   (Hwfpp: OpsemPP.wf_State Cfg1 St1) 
   (Hnoalias: Promotability.wf_State maxb pinfo Cfg1 St1) 
@@ -186,6 +199,182 @@ Lemma dse_is_sim : forall maxb pinfo (sasinfo: SASInfo pinfo) Cfg1 St1 Cfg2 St2
      (Hop1: Opsem.sInsn Cfg1 St1 St1' tr1), 
      State_simulation pinfo sasinfo Cfg1 St1' Cfg2 St2' /\ tr1 = tr2).
 Admitted.
+
+Lemma s_genInitState__sas_State_simulation: forall pinfo sasinfo S1 S2 main 
+  VarArgs cfg2 IS2,
+  system_simulation pinfo sasinfo S1 S2 ->
+  Opsem.s_genInitState S2 main VarArgs Mem.empty = ret (cfg2, IS2) ->
+  exists cfg1, exists IS1,
+    Opsem.s_genInitState S1 main VarArgs Mem.empty = ret (cfg1, IS1) /\
+    State_simulation pinfo sasinfo cfg1 IS1 cfg2 IS2.
+Admitted.
+
+Lemma s_isFinialState__sas_State_simulation: forall pinfo sasinfo cfg1 FS1 cfg2 
+  FS2 r (Hstsim : State_simulation pinfo sasinfo cfg1 FS1 cfg2 FS2)
+  (Hfinal: s_isFinialState cfg2 FS2 = ret r),
+  s_isFinialState cfg1 FS1 = ret r.
+Admitted.
+
+Lemma opsem_s_isFinialState__sas_State_simulation: forall 
+  pinfo sasinfo cfg1 FS1 cfg2 FS2  
+  (Hstsim : State_simulation pinfo sasinfo cfg1 FS1 cfg2 FS2),
+  Opsem.s_isFinialState FS1 = Opsem.s_isFinialState FS2.
+Admitted.
+
+Lemma undefined_state__sas_State_simulation: forall pinfo sasinfo cfg1 St1 cfg2 
+  St2 (Hstsim : State_simulation pinfo sasinfo cfg1 St1 cfg2 St2),
+  OpsemPP.undefined_state cfg1 St1 -> OpsemPP.undefined_state cfg2 St2.
+Admitted.
+
+Lemma sop_star__sas_State_simulation: forall pinfo sasinfo cfg1 IS1 cfg2 IS2 tr
+  FS2 (Hwfpi: WF_PhiInfo pinfo) (Hwfpp: OpsemPP.wf_State cfg1 IS1) maxb
+  (Hnoalias: Promotability.wf_State maxb pinfo cfg1 IS1)
+  (Hstsim : State_simulation pinfo sasinfo cfg1 IS1 cfg2 IS2)
+  (Hopstar : Opsem.sop_star cfg2 IS2 FS2 tr),
+  exists FS1, Opsem.sop_star cfg1 IS1 FS1 tr /\ 
+    State_simulation pinfo sasinfo cfg1 FS1 cfg2 FS2.
+Proof.
+  intros.
+  generalize dependent cfg1.
+  generalize dependent IS1.
+  induction Hopstar; intros.
+    exists IS1. split; auto.
+
+    assert (J:=Hwfpp).
+    apply OpsemPP.progress in J; auto.
+    destruct J as [Hfinal1 | [[IS1' [tr0 Hop1]] | Hundef1]].
+      apply opsem_s_isFinialState__sas_State_simulation in Hstsim.
+      rewrite Hstsim in Hfinal1.
+      contradict H; eauto using s_isFinialState__stuck.
+
+      assert (OpsemPP.wf_State cfg1 IS1') as Hwfpp'.
+        admit. (* wf pp *)
+      assert (Promotability.wf_State maxb pinfo cfg1 IS1') as Hnoalias'.
+        admit. (* wf pp *)
+      eapply sas_is_sim in Hstsim; eauto.
+      destruct Hstsim as [Hstsim1 Hstsim2].
+      destruct (@removable_State_dec pinfo sasinfo IS1) as [Hrm | Hnrm].
+        eapply Hstsim1 in Hrm; eauto.
+        destruct Hrm as [Hstsim EQ]; subst.
+        admit. (* we should do induction on the measure of State_simulation *)
+
+        eapply Hstsim2 in Hnrm; eauto.
+        destruct Hnrm as [Hstsim EQ]; subst.
+        eapply IHHopstar in Hstsim; eauto.
+        destruct Hstsim as [FS1 [Hopstar1 Hstsim]].
+        exists FS1.
+        split; eauto.
+
+      eapply undefined_state__sas_State_simulation in Hstsim; eauto.
+      contradict H; eauto using undefined_state__stuck.
+Qed.
+
+Lemma sop_div__sas_State_simulation: forall pinfo laainfo cfg1 IS1 cfg2 IS2 tr
+  (Hwfpi: WF_PhiInfo pinfo) (Hwfpp: OpsemPP.wf_State cfg1 IS1) maxb
+  (Hnoalias: Promotability.wf_State maxb pinfo cfg1 IS1)
+  (Hstsim : State_simulation pinfo laainfo cfg1 IS1 cfg2 IS2)
+  (Hopstar : Opsem.sop_diverges cfg2 IS2 tr),
+  Opsem.sop_diverges cfg1 IS1 tr.
+Admitted.
+
+Lemma find_st_ld__sasinfo: forall l0 ps0 cs0 tmn0 i0 v cs (pinfo:PhiInfo) dones
+  (Hst : ret inl (i0, v, cs) = find_init_stld cs0 (PI_id pinfo) dones) v0
+  (i1 : id) (Hld : ret inr (i1, v0) = find_next_stld cs (PI_id pinfo))
+  (HBinF : blockInFdefB (block_intro l0 ps0 cs0 tmn0) (PI_f pinfo) = true),
+  exists sasinfo:SASInfo pinfo,
+    SAS_sid1 pinfo sasinfo = i0 /\
+    SAS_sid2 pinfo sasinfo = i1 /\
+    SAS_value1 pinfo sasinfo = v /\
+    SAS_value2 pinfo sasinfo = v0 /\
+    SAS_block pinfo sasinfo = (block_intro l0 ps0 cs0 tmn0).
+Admitted.
+
+Lemma sas_sim: forall (los : layouts) (nts : namedts) (fh : fheader) 
+  (dones : list id) (pinfo : PhiInfo) (main : id) (VarArgs : list (GVsT DGVs))
+  (bs1 : list block) (l0 : l) (ps0 : phinodes) (cs0 : cmds) (tmn0 : terminator)
+  (bs2 : list block) (Ps1 : list product) (Ps2 : list product) (i0 : id)
+  (v : value) (cs : cmds) 
+  (Hst1 : ret inl (i0, v, cs) = find_init_stld cs0 (PI_id pinfo) dones)
+  (i1 : id) (v0 : value)
+  (Hst2 : ret inr (i1, v0) = find_next_stld cs (PI_id pinfo))
+  (Heq: PI_f pinfo = fdef_intro fh (bs1 ++ block_intro l0 ps0 cs0 tmn0 :: bs2))
+  (Hwfpi: WF_PhiInfo pinfo) 
+  (HwfS : 
+     wf_system nil
+       [module_intro los nts 
+         (Ps1 ++ 
+          product_fdef 
+            (fdef_intro fh (bs1 ++ block_intro l0 ps0 cs0 tmn0 :: bs2))
+          :: Ps2)]),
+  program_sim
+    [module_intro los nts
+      (Ps1 ++
+       product_fdef
+         (fdef_intro fh
+           (List.map (remove_block i0)
+             (bs1 ++ block_intro l0 ps0 cs0 tmn0 :: bs2))) :: Ps2)]
+    [module_intro los nts
+      (Ps1 ++
+       product_fdef
+         (fdef_intro fh (bs1 ++ block_intro l0 ps0 cs0 tmn0 :: bs2)) :: Ps2)]
+    main VarArgs.
+Proof.
+  intros.
+  assert (blockInFdefB (block_intro l0 ps0 cs0 tmn0) (PI_f pinfo) = true)
+    as HBinF.
+    rewrite Heq. simpl. apply InBlocksB_middle.
+  eapply find_st_ld__sasinfo in HBinF; eauto.
+  destruct HBinF as [sasinfo [J1 [J2 [J3 [J4 J5]]]]]; subst.
+  assert (Huniq:=HwfS). apply wf_system__uniqSystem in Huniq; auto.
+  assert (system_simulation pinfo sasinfo
+     [module_intro los nts
+        (Ps1 ++
+         product_fdef
+           (fdef_intro fh (bs1 ++ block_intro l0 ps0 cs0 tmn0 :: bs2)) :: Ps2)]
+     [module_intro los nts
+        (Ps1 ++
+         product_fdef
+           (remove_fdef (SAS_sid1 pinfo sasinfo)
+              (fdef_intro fh (bs1 ++ block_intro l0 ps0 cs0 tmn0 :: bs2)))
+         :: Ps2)]) as Hssim.
+    unfold system_simulation.
+    constructor; auto.
+    repeat split; auto.
+    unfold products_simulation.
+    simpl in Huniq. destruct Huniq as [[_ [_ Huniq]] _].
+    apply uniq_products_simulation; auto.
+  constructor.
+    intros tr t Hconv.
+    inv Hconv.
+    eapply s_genInitState__sas_State_simulation in H; eauto.
+    destruct H as [cfg1 [IS1 [Hinit Hstsim]]].    
+    assert (OpsemPP.wf_State cfg1 IS1) as Hwfst. 
+      eapply s_genInitState__opsem_wf; eauto.
+    assert (exists maxb, 
+              MemProps.wf_globals maxb (OpsemAux.Globals cfg1) /\ 0 <= maxb /\
+              Promotability.wf_State maxb pinfo cfg1 IS1) as Hprom.
+      eapply Promotability.s_genInitState__wf_globals_promotable; eauto.
+    destruct Hprom as [maxb [Hwfg [Hless Hprom]]].
+    eapply sop_star__sas_State_simulation in Hstsim; eauto.
+    destruct Hstsim as [FS1 [Hopstar1 Hstsim']].
+    eapply s_isFinialState__sas_State_simulation in Hstsim'; eauto.
+    econstructor; eauto.
+
+    intros tr Hdiv.
+    inv Hdiv.
+    eapply s_genInitState__sas_State_simulation in H; eauto.
+    destruct H as [cfg1 [IS1 [Hinit Hstsim]]].  
+    assert (OpsemPP.wf_State cfg1 IS1) as Hwfst. 
+      eapply s_genInitState__opsem_wf; eauto.
+    assert (exists maxb, 
+              MemProps.wf_globals maxb (OpsemAux.Globals cfg1) /\ 0 <= maxb /\
+              Promotability.wf_State maxb pinfo cfg1 IS1) as Hprom.
+      eapply Promotability.s_genInitState__wf_globals_promotable; eauto.
+    destruct Hprom as [maxb [Hwfg [Hless Hprom]]].
+    eapply sop_div__sas_State_simulation in Hstsim; eauto.
+    destruct Hstsim as [FS1 Hopdiv1].
+    econstructor; eauto.
+Qed.
 
 (*****************************)
 (*
